\documentclass{article}

\usepackage[left=1in, right=1in, top=1in, bottom=1in]{geometry}
\usepackage{amsfonts}
\usepackage{amsmath}
\usepackage{amssymb}
\usepackage{amsthm}


\begin{document}
\pagenumbering{gobble}

\section*{Fibonacci Sequence Closed Form}

The Fibonacci sequence $F_n$ is defined as follows.
\begin{align*}
  F_0 &= 0, &
  F_1 &= 1, &
  F_{n+2} &= F_{n+1} + F_n.
\end{align*}

\paragraph{Theorem.}
The Fibonacci sequence has closed closed formula, dubbed $h_n$, defined as
\begin{align*}
  h_n = \frac{1}{\sqrt{5}} \left(\phi_+^{n+1} - \phi_-^{n+1}\right)
  =
  \frac{1}{\sqrt{5}} \left(\phi_+^n - \phi_-^n\right).
\end{align*}
where
$\phi_+ = \frac{1 + \sqrt{5}}{2}$ and
$\phi_- = \frac{1 + \sqrt{5}}{2}$.
where
\begin{align*}
  \phi_+ &= \frac{1 + \sqrt{5}}{2}, &
  \phi_- &= \frac{1 + \sqrt{5}}{2}.
\end{align*}

\begin{proof}
Consider the infinite $x$-power series
\begin{align*}
\tag{\texttt{f\textsubscript{0}}}
  f = \sum_{i=0}^\infty F_{i+1} x^i
\end{align*}
and suppose $0 < x < 1/2$ (e.g. $1/4$).
Then
\begin{align*}
\tag{\texttt{g\textsubscript{1}}}
  (1 - x - x^2) f
&=
  \sum_{i=0}^\infty (1 - x - x^2) F_{i+1} x^i
\\&=
  \sum_{i=0}^\infty F_{i+1} (x^i - x^{i+1} - x^{i+2})
\\&=
  (F_1 x^0 - F_1 x^1 - F_1 x^2) +
  (F_2 x^1 - F_2 x^2 - F_2 x^3) +
  (F_3 x^2 - F_3 x^3 - F_3 x^4) + \cdots
\\&=
\tag{\texttt{g\textsubscript{2}}}
  F_1 x^0 +
  (F_2 - F_1) x^1 +
  (F_3 - F_1 - F_2) x^2 +
  (F_4 - F_2 - F_3) x^3 +
  \cdots
\\&=
\tag{\texttt{g\textsubscript{3}}}
  1 x^0 +
  0 x^1 +
  ((F_1 + F_2) - F_1 - F_2) x^2 +
  ((F_2 + F_3) - F_2 - F_3) x^3 +
  \cdots
\\&=
  1 +
  0 +
  0 x^2 +
  0 x^3 +
  \cdots
\\&=
\tag{\texttt{g\textsubscript{4}}}
  1
\\\implies
  f
&=
\tag{\texttt{f\textsubscript{1}}}
  \frac{1}{1 - x - x^2}
\\&=
\tag{\texttt{f\textsubscript{2}}}
  \frac{1}{\sqrt{5}} \left(
    \frac{\phi_+}{1 - \phi_+} -
    \frac{\phi_-}{1 - \phi_-}
  \right).
\end{align*}
Since for $|x| < 1/2$, $\frac{1}{(1 - a x)} = \sum_{i=0}^\infty (a x)^n$,
we have
\begin{align*}
  f
=
  \frac{1}{\sqrt{5}} \left(
    \frac{\phi_+}{1 - \phi_+} -
    \frac{\phi_-}{1 - \phi_-}
  \right)
&=
\tag{\texttt{f\textsubscript{3}}}
  \frac{1}{\sqrt{5}} \left(
    \left(\phi_+ \sum_{i=0}^\infty \phi_+^i x^i\right) -
    \left(\phi_-\sum_{i=0}^\infty \phi_-^i x^i\right)
  \right)
\\&=
\tag{\texttt{f\textsubscript{4}}}
  \sum_{i=0}^\infty \left(
    \frac{1}{\sqrt{5}} \left(\phi_+^{i+1} - \phi_-^{i+1}\right) x^i
  \right)
\\\implies
  \sum_{i=0}^\infty F_{i+1} x^i
&=
% \tag{\texttt{f\textsubscript{0 \approx f_4}}}
\tag{$\texttt{f\textsubscript{0}} \approx \texttt{f\textsubscript{4}}$}
  \sum_{i=0}^\infty \left(
    \frac{1}{\sqrt{5}} \left(\phi_+^{i+1} - \phi_-^{i+1}\right) x^i
  \right)
\\\implies
\tag{$F_{n+1} \equiv h_{n+1}$}
\forall n,
  F_{n+1}
&=
  \frac{1}{\sqrt{5}} \left(\phi_+^{n+1} - \phi_-^{n+1}\right)
=
  h_{n+1}
\\\implies
\tag{$F_{n} \equiv h_{n}$}
\forall n,
  F_n
&=
  h_n.
\end{align*}
\end{proof}
\end{document}
